generational/spec/GC.Gen.CheneyCorrectness.fst
@@ -232,6 +232,7 @@ let chunked_cheney_gc_correct_after_preflight
        collect.cmc_roots == rewrite_roots roots prom.fwd_map /\
        collect.cmc_fwd == prom.fwd_map /\
        CheneyPres.chunked_fwd_targets_above_minor collect.cmc_fwd /\
+       CheneyPres.chunked_fwd_targets_valid_addr collect.cmc_fwd /\
        GenInv.chunked_major_alloc_shape
         collect.cmc_major collect.cmc_fp r.capacity_fuel_out /\
        SpecMajorAlloc.major_fl_chain_terminates
