spot/GC.SPOT.HeapExpansion.fst
@@ -1822,6 +1822,7 @@ let spot_chunked_cheney_promote_after_minor_promotion_head_preflight
          GenInv.chunked_chain_objects_blue
            r.capacity_major_out r.capacity_fp_out r.capacity_fuel_out /\
          CheneyPreservation.chunked_fwd_targets_above_minor res.fwd_map /\
+         CheneyPreservation.chunked_fwd_targets_valid_addr res.fwd_map /\
          (forall (x:U64.t).
            Seq.mem x (minor_reachable minor roots) /\
            minor_wosize minor x > 0 ==>
@@ -3542,6 +3543,7 @@ let spot_chunked_cheney_collect_after_minor_promotion_head_preflight
          collect.cmc_roots == rewrite_roots roots prom.fwd_map /\
          collect.cmc_fwd == prom.fwd_map /\
          CheneyPreservation.chunked_fwd_targets_above_minor collect.cmc_fwd /\
+         CheneyPreservation.chunked_fwd_targets_valid_addr collect.cmc_fwd /\
          GenInv.chunked_major_alloc_shape
            collect.cmc_major collect.cmc_fp r.capacity_fuel_out /\
          SpecMajorAlloc.major_fl_chain_terminates
@@ -3667,6 +3669,7 @@ let spot_chunked_cheney_gc_correct_after_preflight
          collect.cmc_roots == rewrite_roots roots prom.fwd_map /\
          collect.cmc_fwd == prom.fwd_map /\
          CheneyPreservation.chunked_fwd_targets_above_minor collect.cmc_fwd /\
+         CheneyPreservation.chunked_fwd_targets_valid_addr collect.cmc_fwd /\
          GenInv.chunked_major_alloc_shape
            collect.cmc_major collect.cmc_fp r.capacity_fuel_out /\
          SpecMajorAlloc.major_fl_chain_terminates
